Minimmit/Model/Transition/Execute.lean
@@ -1,4 +1,4 @@
-import Minimmit.Model.Transition
+import Minimmit.Model.Transition.Basic
 
 /-!
 # 遷移系の補題
